added the notion of subsumption rule for effects in type system

cfrontend/BeePL_typesystem.v
@@ -10,30 +10,26 @@ Definition empty_effect : effect := nil.
 Definition type_bool (t : type) : Prop :=
 classify_bool t <> bool_default.
 
-
 Inductive type_expr : ty_context -> store_context -> expr -> effect -> type -> Prop :=
 (*For all value expression, we can assume any effect type, including the empty effect *)
-| ty_valu : forall Gamma Sigma ef,
-            type_expr Gamma Sigma (Val Vunit (Ptype Tunit)) ef (Ptype Tunit)
-| ty_vali : forall Gamma Sigma ef i sz s a,
-            type_expr Gamma Sigma (Val (Vint i) (Ptype (Tint sz s a))) ef (Ptype (Tint sz s a))
-| ty_vall : forall Gamma Sigma ef i s a,
-            type_expr Gamma Sigma (Val (Vint64 i) (Ptype (Tlong s a))) ef (Ptype (Tlong s a))
-| ty_valloc : forall Gamma Sigma ef l ofs h t a,
+| ty_valu : forall Gamma Sigma,
+            type_expr Gamma Sigma (Val Vunit (Ptype Tunit)) nil (Ptype Tunit)
+| ty_vali : forall Gamma Sigma i sz s a,
+            type_expr Gamma Sigma (Val (Vint i) (Ptype (Tint sz s a))) nil (Ptype (Tint sz s a))
+| ty_vall : forall Gamma Sigma i s a,
+            type_expr Gamma Sigma (Val (Vint64 i) (Ptype (Tlong s a))) nil (Ptype (Tlong s a))
+| ty_valloc : forall Gamma Sigma l ofs h t a,
               PTree.get l Sigma = Some (Reftype h t a) ->
-              type_expr Gamma Sigma (Val (Vloc l ofs) (Reftype h t a)) ef (Reftype h t a)
+              type_expr Gamma Sigma (Val (Vloc l ofs) (Reftype h t a)) nil (Reftype h t a)
 | ty_var : forall Gamma Sigma x t, 
            PTree.get x (extend_context Gamma x t) = Some t ->
-           type_expr Gamma Sigma (Var x t) empty_effect t
-| ty_constint : forall Gamma Sigma t sz s a i,
-                t = (Ptype (Tint sz s a)) ->
-                type_expr Gamma Sigma (Const (ConsInt i) t) empty_effect t
-| ty_constlong : forall Gamma Sigma t s a i,
-                 t = (Ptype (Tlong s a)) ->
-                 type_expr Gamma Sigma (Const (ConsLong i) t) empty_effect t
-| ty_constunit : forall Gamma Sigma t,
-                 t = (Ptype Tunit) ->
-                 type_expr Gamma Sigma (Const (ConsUnit) t) empty_effect t
+           type_expr Gamma Sigma (Var x t) nil t
+| ty_constint : forall Gamma Sigma sz s a i,
+                type_expr Gamma Sigma (Const (ConsInt i) (Ptype (Tint sz s a))) nil (Ptype (Tint sz s a))
+| ty_constlong : forall Gamma Sigma s a i,
+                 type_expr Gamma Sigma (Const (ConsLong i) (Ptype (Tlong s a))) nil (Ptype (Tlong s a))
+| ty_constunit : forall Gamma Sigma,
+                 type_expr Gamma Sigma (Const (ConsUnit) (Ptype Tunit)) nil (Ptype Tunit)
 (* Fix me *)
 | ty_app : forall Gamma Sigma e es rt efs ts ef efs', 
            type_expr Gamma Sigma e ef (Ftype ts efs rt) -> 
@@ -67,15 +63,12 @@ Inductive type_expr : ty_context -> store_context -> expr -> effect -> type -> P
             type_expr Gamma Sigma e ef t ->
             type_expr (extend_context Gamma x t) Sigma e' ef' t' ->
             type_expr Gamma Sigma (Bind x t e e' t') (ef ++ ef') t'
-| ty_cond : forall Gamma Sigma e1 e2 e3 tb t ef1 ef2 ef3 ef1' ef, 
+| ty_cond : forall Gamma Sigma e1 e2 e3 tb t ef1 ef2, 
             type_expr Gamma Sigma e1 ef1 tb ->
-            sub_effect ef1 ef1' ->
             type_bool tb ->
             type_expr Gamma Sigma e2 ef2 t ->
-            sub_effect ef2 ef = true ->
-            type_expr Gamma Sigma e3 ef3 t ->
-            sub_effect ef3 ef = true ->
-            type_expr Gamma Sigma (Cond e1 e2 e3 t) (ef1' ++ ef) t
+            type_expr Gamma Sigma e3 ef2 t ->
+            type_expr Gamma Sigma (Cond e1 e2 e3 t) (ef1 ++ ef2) t
 | ty_unit : forall Gamma Sigma,
             type_expr Gamma Sigma (Unit (Ptype Tunit)) empty_effect (Ptype Tunit)
 | ty_addr : forall Gamma Sigma l ofs h t a,
@@ -83,13 +76,17 @@ Inductive type_expr : ty_context -> store_context -> expr -> effect -> type -> P
             (*t' = (Reftype h t a) ->*)
             type_expr Gamma Sigma (Addr l ofs (Reftype h t a)) empty_effect (Reftype h t a) 
 (* return type, arg types, and effect must agree with the signature
-   eBPF helper functions never return a void type  *)
+   eBPF helper functions never return a void type and a function  *)
 | ty_ext : forall Gamma Sigma exf ts es ef rt,
            rt = get_rt_eapp exf ->
            rt <> Ptype Tunit /\ is_funtype rt = false -> 
            ts = get_at_eapp exf ->
            type_exprs Gamma Sigma es ef ts ->
            type_expr Gamma Sigma (Eapp exf ts es rt) ((get_ef_eapp exf) ++ ef) rt
+| ty_sub : forall Gamma Sigma e ef t ef', 
+           type_expr Gamma Sigma e ef t ->
+           sub_effect ef ef' ->
+           type_expr Gamma Sigma e ef' t
 (* fix me : Run *)
 (* fix me : Hexpr *)
 (*| ty_hexpr : forall Gamma Sigma m e h ef t a, 
@@ -108,6 +105,127 @@ Scheme type_expr_ind_mut := Induction for type_expr Sort Prop
   with type_exprs_ind_mut := Induction for type_exprs Sort Prop.
 Combined Scheme type_exprs_type_expr_ind_mut from type_exprs_ind_mut, type_expr_ind_mut.
 
+
+(*Inductive type_expr : ty_context -> store_context -> expr -> effect -> type -> Prop :=
+(*For all value expression, we can assume any effect type, including the empty effect *)
+| ty_valu : forall Gamma Sigma ef,
+            type_expr Gamma Sigma (Val Vunit (Ptype Tunit)) ef (Ptype Tunit)
+| ty_vali : forall Gamma Sigma ef i sz s a,
+            type_expr Gamma Sigma (Val (Vint i) (Ptype (Tint sz s a))) ef (Ptype (Tint sz s a))
+| ty_vall : forall Gamma Sigma ef i s a,
+            type_expr Gamma Sigma (Val (Vint64 i) (Ptype (Tlong s a))) ef (Ptype (Tlong s a))
+| ty_valloc : forall Gamma Sigma ef l ofs h t a,
+              PTree.get l Sigma = Some (Reftype h t a) ->
+              type_expr Gamma Sigma (Val (Vloc l ofs) (Reftype h t a)) ef (Reftype h t a)
+| ty_var : forall Gamma Sigma x t ef, 
+           PTree.get x (extend_context Gamma x t) = Some t ->
+           sub_effect nil ef ->
+           type_expr Gamma Sigma (Var x t) ef t
+| ty_consti : forall Gamma Sigma sz s a i ef,
+              sub_effect nil ef ->
+              type_expr Gamma Sigma (Const (ConsInt i) (Ptype (Tint sz s a))) ef (Ptype (Tint sz s a))
+| ty_constl : forall Gamma Sigma s a i ef,
+              sub_effect nil ef ->
+              type_expr Gamma Sigma (Const (ConsLong i) (Ptype (Tlong s a))) ef (Ptype (Tlong s a))
+| ty_constu : forall Gamma Sigma ef,
+              sub_effect nil ef ->
+              type_expr Gamma Sigma (Const (ConsUnit) (Ptype Tunit)) ef (Ptype Tunit)
+(* Fix me *)
+| ty_app : forall Gamma Sigma e es rt efs ts ef efb ef' efs' efb' ef1, 
+           type_expr Gamma Sigma e ef (Ftype ts efs rt) -> 
+           sub_effect ef ef' ->
+           sub_effect efs efs' ->
+           type_exprs Gamma Sigma es efb ts ->
+           sub_effect efb efb' ->
+           sub_effect (ef' ++ efs' ++ efb') ef1 ->
+           type_expr Gamma Sigma (App e es rt) ef1 rt
+| ty_ref : forall Gamma Sigma e ef h bt a ef' ef'', 
+           type_expr Gamma Sigma e ef (Ptype bt) ->
+           sub_effect ef ef' ->
+           sub_effect (ef' ++ (Alloc h :: nil)) ef'' ->
+           type_expr Gamma Sigma (Prim Ref (e::nil) (Reftype h (Bprim bt) a)) ef'' (Reftype h (Bprim bt) a)
+| ty_deref : forall Gamma Sigma e ef h bt a ef' ef'', (* inner expression should be unrestricted as it will be used later *)
+             type_expr Gamma Sigma e ef (Reftype h (Bprim bt) a) -> 
+             sub_effect ef ef' ->
+             sub_effect (ef' ++ (Read h :: nil)) ef'' ->
+             type_expr Gamma Sigma (Prim Deref (e::nil) (Ptype bt)) ef'' (Ptype bt)
+| ty_massgn : forall Gamma Sigma e1 e2 h bt ef1 a ef2 ef1' ef2' ef, 
+              type_expr Gamma Sigma e1 ef1 (Reftype h (Bprim bt) a) ->
+              sub_effect ef1 ef1' ->
+              type_expr Gamma Sigma e2 ef2 (Ptype bt) ->
+              sub_effect ef2 ef2' ->
+              sub_effect (ef1' ++ ef2' ++ (Write h :: nil)) ef ->
+              type_expr Gamma Sigma (Prim Massgn (e1::e2::nil) (Ptype Tunit)) ef (Ptype Tunit)
+| ty_uop : forall Gamma Sigma op e ef t ef',
+           is_reftype t = false ->
+           is_unittype t = false ->
+           type_expr Gamma Sigma e ef t ->
+           sub_effect ef ef' ->
+           type_expr Gamma Sigma (Prim (Uop op) (e::nil) t) ef' t
+| ty_bop : forall Gamma Sigma op e ef t e' ef',
+           is_reftype t = false ->
+           is_unittype t = false ->
+           type_expr Gamma Sigma e ef t ->
+           type_expr Gamma Sigma e' ef t ->
+           sub_effect ef ef' ->
+           type_expr Gamma Sigma (Prim (Bop op) (e::e'::nil) t) ef' t 
+| ty_bind : forall Gamma Sigma x t e e' t' ef1 ef2 ef,
+            type_expr Gamma Sigma e ef1 t ->
+            type_expr (extend_context Gamma x t) Sigma e' ef2 t' ->
+            sub_effect (ef1 ++ ef2) ef ->
+            type_expr Gamma Sigma (Bind x t e e' t') ef t'
+| ty_cond : forall Gamma Sigma e1 e2 e3 tb t ef1 ef2 ef3 ef1' ef, 
+            type_expr Gamma Sigma e1 ef1 tb ->
+            sub_effect ef1 ef1' ->
+            type_bool tb ->
+            type_expr Gamma Sigma e2 ef2 t ->
+            sub_effect ef2 ef = true ->
+            type_expr Gamma Sigma e3 ef3 t ->
+            sub_effect ef3 ef = true ->
+            (*sub_effect (ef1' ++ ef) ef' ->*)
+            type_expr Gamma Sigma (Cond e1 e2 e3 t) (ef1' ++ ef) t
+| ty_unit : forall Gamma Sigma ef,
+            type_expr Gamma Sigma (Unit (Ptype Tunit)) nil (Ptype Tunit) ->
+            sub_effect nil ef ->
+            type_expr Gamma Sigma (Unit (Ptype Tunit)) ef (Ptype Tunit)
+| ty_addr : forall Gamma Sigma l ofs h t a ef,
+            PTree.get l.(lname) Sigma = Some (Reftype h t a) ->
+            type_expr Gamma Sigma (Addr l ofs (Reftype h t a)) nil (Reftype h t a) ->
+            sub_effect nil ef -> 
+            type_expr Gamma Sigma (Addr l ofs (Reftype h t a)) ef (Reftype h t a)
+(* return type, arg types, and effect must agree with the signature
+   eBPF helper functions never return a void type  *)
+| ty_ext : forall Gamma Sigma exf ts es ef rt ef' ef'',
+           rt = get_rt_eapp exf ->
+           rt <> Ptype Tunit /\ is_funtype rt = false -> 
+           ts = get_at_eapp exf ->
+           type_exprs Gamma Sigma es ef ts ->
+           sub_effect ef ef' ->
+           sub_effect ((get_ef_eapp exf) ++ ef') ef'' ->
+           type_expr Gamma Sigma (Eapp exf ts es rt) ef'' rt
+(* fix me : Run *)
+(* fix me : Hexpr *)
+(*| ty_hexpr : forall Gamma Sigma m e h ef t a, 
+             type_expr Gamma Sigma e ef (Reftype h (Bprim t) a) ->
+             type_expr Gamma Sigma (Hexpr m e (Reftype h (Bprim t) a)) ef (Reftype h (Bprim t) a)*)
+(* fix me : Add typing rule for external function *)
+with type_exprs : ty_context -> store_context -> list expr -> effect -> list type -> Prop :=
+| ty_nil : forall Gamma Sigma ef,
+           type_exprs Gamma Sigma nil nil nil ->
+           sub_effect nil ef ->
+           type_exprs Gamma Sigma nil ef nil
+| ty_cons : forall Gamma Sigma e es ef efs t ts ef' efs' ef'',
+            type_expr Gamma Sigma e ef t ->
+            sub_effect ef ef' ->
+            type_exprs Gamma Sigma es efs ts ->
+            sub_effect efs efs' ->
+            sub_effect (ef' ++ efs') ef'' ->
+            type_exprs Gamma Sigma (e :: es) ef'' (t :: ts).
+           
+Scheme type_expr_ind_mut := Induction for type_expr Sort Prop
+  with type_exprs_ind_mut := Induction for type_exprs Sort Prop.
+Combined Scheme type_exprs_type_expr_ind_mut from type_exprs_ind_mut, type_expr_ind_mut.*)
+
 (* The (EXTEND) rule states that we can always assume a worse effect; 
    this rule is not part of the inference rules but
    we need it to show subject reduction of stateful computations. : Leijen's koka paper *)
@@ -122,7 +240,114 @@ sub_effect ef ef = true.
 Proof.
 Admitted.
 
-Section type_expr_ind.
+(* Complete Me: Easy *)
+Lemma sub_effect_nil : forall ef, 
+sub_effect nil ef = true.
+Proof.
+Admitted.
+
+(* Complete Me: Easy *)
+Lemma sub_effect_trans : forall ef1 ef2 ef3, 
+sub_effect ef1 ef2 = true ->
+sub_effect ef2 ef3 = true ->
+sub_effect ef1 ef3 = true.
+Proof.
+Admitted.
+
+(*Lemma extend_effect : 
+(forall Gamma Sigma es efs ts efs', type_exprs Gamma Sigma es efs ts ->
+                                    sub_effect efs efs' ->
+                                    type_exprs Gamma Sigma es efs' ts) /\
+(forall Gamma Sigma e ef t ef', type_expr Gamma Sigma e ef t ->
+                                sub_effect ef ef' ->
+                                type_expr Gamma Sigma e ef' t).
+Proof.
+suff : (forall Gamma Sigma es efs ts, type_exprs Gamma Sigma es efs ts ->
+                                      forall efs', sub_effect efs efs' -> 
+                                                   type_exprs Gamma Sigma es efs' ts) /\
+       (forall Gamma Sigma e ef t, type_expr Gamma Sigma e ef t ->
+                                   forall ef', sub_effect ef ef' ->
+                                               type_expr Gamma Sigma e ef' t).
++ move=> [] hin hin'. split=> //=.
+  + move=> Gamma Sigma es efs ts efs' hts hs.
+    by move: (hin Gamma Sigma es efs ts hts efs' hs).
+  move=> Gamma Sigma e ef t ef' ht hs.
+  by move: (hin' Gamma Sigma e ef t ht ef' hs).
+apply type_exprs_type_expr_ind_mut=> //=.
+(* val unit *)
++ move=> Gamma Sigma ef ef' hs. by apply ty_valu.
+(* val int *)
++ move=> Gamma Sigma ef ef' i sz s a hs. by apply ty_vali.
+(* val long *)
++ move=> Gamma Sigma ef ef' i s a hs. by apply ty_vall.
+(* val loc *)
++ move=> Gamma Sigma ef l ofs h t a hsi ef' hs. by apply ty_valloc.
+(* var *)
++ move=> Gamma Sigma x t ef hte _ ef' hs. by apply ty_var.
+(* const int *)
++ move=> Gamma Sigma sz s a i ef _ ef' hs. by apply ty_consti.
+(* const long *)
++ move=> Gamma Sigma s a i ef _ ef' hs. by apply ty_constl.
+(* const unit *)
++ move=> Gamma Sigma ef _ ef' hs. by apply ty_constu.
+(* app *)
++ move=> Gamma Sigma e es rt efs ts ef efb ef' efs' efb' ef1 
+  hte hin hs1 hs2 htes hin' hs3 hs4 ef2 hs5.
+  apply ty_app with efs ts ef efb ef' efs' efb'.
+  + by apply hte. + by apply hs1. + by apply hs2. + by apply htes.
+  + by apply hs3. 
+  by have := sub_effect_trans (ef' ++ efs' ++ efb') ef1 ef2 hs4 hs5.
+(* ref *)
++ move=> Gamma Sigma e ef h bt a ef' ef'' hte hin hs hs' ef''' hs''.
+  apply ty_ref with ef ef'.
+  + by apply hte.
+  + by apply hs.
+  by have := sub_effect_trans (ef' ++ [:: Alloc h]) ef'' ef''' hs' hs''.
+(* deref *)
++ move=> Gamma Sigma e ef h bt a ef' ef'' ht hin hs1 hs2 ef1 hs3. 
+  apply ty_deref with ef h a ef'. + by apply ht. by apply hs1.
+  by have := sub_effect_trans (ef' ++ [:: Read h]) ef'' ef1 hs2 hs3.
+(* massgn *)
++ move=> Gamma Sigma e1 e2 h bt ef1 a ef2 ef1' ef2' ef ht1 hin hs1 ht2 hin' hs2 hs3 ef' hs'.
+  apply ty_massgn with h bt ef1 a ef2 ef1' ef2'. + by apply ht1. + by apply hs1.
+  + by apply ht2. + by apply hs2. 
+  by have := sub_effect_trans (ef1' ++ ef2' ++ [:: Write h]) ef ef' hs3 hs'.
+(* uop *)
++ move=> Gamma Sigma op e ef t ef' hrt hut ht hin hs1 ef'' hs2.
+  apply ty_uop with ef. + by apply hrt. + by apply hut. + by apply ht. 
+  by have := sub_effect_trans ef ef' ef'' hs1 hs2.
+(* bop *)
++ move=> Gamma Sigma op e ef t e' ef' hrt hut ht hin ht' hin' hs1 ef'' hs2.
+  apply ty_bop with ef. + by apply hrt. + by apply hut. + by apply ht. + by apply ht'.
+  by have := sub_effect_trans ef ef' ef'' hs1 hs2.
+(* bind *)
++ move=> Gamma Sigma x t e e' t' ef1 ef2 ef ht hin ht' hin' hs2 ef' hs3.
+  apply ty_bind with ef1 ef2. + by apply ht. + by apply ht'.
+  by have := sub_effect_trans (ef1 ++ ef2) ef ef' hs2 hs3.
+(* cond *)
++ move=> Gamma Sigma e1 e2 e3 tb t ef1 ef2 ef3 ef1' ef ht1 hin1 
+         hs1 htb ht2 hin2 hs2 hs3 ht3 hin3 eff hs.
+  apply ty_cond with tb ef1 ef2 ef3 ef1' ef. + by apply ht1.
+  + by apply hs1. + by apply htb. + by apply ht2. + by apply hs2.
+  + by apply ht3. + by apply hs3.
+  by have := sub_effect_trans (ef1' ++ ef) ef' ef'' hs4 hs5.
+(* unit *)
++ move=> Gamma Sigma ef ht hin _ ef' hs. by apply ty_unit.
+(* addr *)
++ move=> Gamma Sigma l ofs h t a ef hsig ht hin _ ef' hs. by apply ty_addr.
+(* eapp *)
++ move=> Gamma Sigma exf ts es ef rt ef' ef'' hrt [] h1 h2 hts htes hin hs1 hs2 ef1 hs3.
+  apply ty_ext with ef ef'; auto. 
+  by have := sub_effect_trans (get_ef_eapp exf ++ ef') ef'' ef1 hs2 hs3.
+(* nil *)
++ move=> Gamma Sigma ef ht hin _ efs' hs. by apply ty_nil.
+(* cons *)
+move=> Gamma Sigma e es ef efs t ts ef' efs' ef'' ht hin hs hts hin' hs1 hs2 efs'' hs3.
+apply ty_cons with ef efs ef' efs'; auto. 
+by have := sub_effect_trans (ef' ++ efs') ef'' efs'' hs2 hs3.
+Qed.*)
+
+(*Section type_expr_ind.
 Context (Pts : ty_context -> store_context -> list expr -> effect -> list type -> Prop).
 Context (Pt : ty_context -> store_context -> expr -> effect -> type -> Prop).
 Context (Htvalu : forall Gamma Sigma ef,
@@ -253,7 +478,201 @@ move=> Gamma Sigma e es ef efs t ts hte ht htes hts.
 by apply Htcons.
 Qed.
 
-End type_expr_ind.
+End type_expr_ind.*)
+
+
+(* Value typing *)
+(* A value does not produce any effect *)
+Lemma value_typing : forall Gamma Sigma ef t v,
+type_expr Gamma Sigma (Val v t) ef t ->
+type_expr Gamma Sigma (Val v t) nil t. 
+Proof.
+move=> Gamma Sigma ef t v. move eq : (Val v t)=> v' ht.
+elim: ht eq=> //=.
++ move=> Gamma' Sigma' [] h1; subst. by apply ty_valu.
++ move=> Gamma' Sigma' i sz s a [] h1; subst. by apply ty_vali.
++ move=> Gamma' Sigma' i s a [] h1; subst. by apply ty_vall.
+move=> Gamma' Sigma' l ofs h bt a hs [] h1; subst. by apply ty_valloc. 
+Qed.
+
+Lemma type_infer_vunit: forall Gamma Sigma ef t, 
+type_expr Gamma Sigma (Val Vunit (Ptype Tunit)) ef t ->
+Ptype Tunit = t.
+Proof.
+move=> Gamma Sigma ef t. 
+move eq : (Val Vunit (Ptype Tunit))=> v ht. elim: ht eq=>//=.
+Qed.
+
+Lemma type_infer_int: forall Gamma Sigma ef t i sz s a, 
+type_expr Gamma Sigma (Val (Vint i) (Ptype (Tint sz s a))) ef t ->
+Ptype (Tint sz s a) = t.
+Proof.
+move=> Gamma Sigma ef t i sz s a. 
+move eq : (Val (Vint i) (Ptype (Tint sz s a)))=> v ht. 
+elim: ht eq=>//=. by move=> Gamma' Sigma' i' sz' s' a' [] h1 h2 h3 h4; subst.
+Qed.
+
+Lemma type_infer_long: forall Gamma Sigma ef t i s a, 
+type_expr Gamma Sigma (Val (Vint64 i) (Ptype (Tlong s a))) ef t ->
+Ptype (Tlong s a) = t.
+Proof.
+move=> Gamma Sigma ef t i s a. 
+move eq : (Val (Vint64 i) (Ptype (Tlong s a)))=> v ht. 
+elim: ht eq=>//=. by move=> Gamma' Sigma' i' s' a' [] h2 h3 h4; subst.
+Qed.
+
+Lemma type_infer_loc: forall Gamma Sigma ef t h bt a l ofs, 
+type_expr Gamma Sigma (Val (Vloc l ofs) (Reftype h bt a)) ef t ->
+(Reftype h bt a) = t.
+Proof.
+move=> Gamma Sigma ef t h bt a l ofs. 
+move eq : (Val (Vloc l ofs) (Reftype h bt a))=> v ht. elim: ht eq=>//=.
+by move=> Gamma' Sigma' l' ofs' h' bt' a' hs [] h1 h2 h3 h4 h5; subst. 
+Qed.
+
+Lemma type_infer_var : forall Gamma Sigma x t ef t',
+type_expr Gamma Sigma (Var x t) ef t' ->
+t = t'.
+Proof.
+move=> Gamma Sigma x t ef t'. 
+move eq: (Var x t)=> v ht. elim: ht eq=> //=.
+by move=> Gamma' Sigma' x' t'' hxt [] h1 h2; subst.
+Qed.
+
+Lemma type_infer_consti: forall Gamma Sigma ef t i sz s a, 
+type_expr Gamma Sigma (Const (ConsInt i) (Ptype (Tint sz s a))) ef t ->
+Ptype (Tint sz s a) = t.
+Proof.
+move=> Gamma Sigma ef t i sz s a. 
+move eq : (Const (ConsInt i) (Ptype (Tint sz s a)))=> v ht. 
+elim: ht eq=>//=. by move=> Gamma' Sigma' i' sz' s' a' [] h1 h2 h3 h4; subst.
+Qed.
+
+Lemma type_infer_constl: forall Gamma Sigma ef t i s a, 
+type_expr Gamma Sigma (Const (ConsLong i) (Ptype (Tlong s a))) ef t ->
+Ptype (Tlong s a) = t.
+Proof.
+move=> Gamma Sigma ef t i s a. 
+move eq : (Const (ConsLong i) (Ptype (Tlong s a)))=> v ht. 
+elim: ht eq=>//=. by move=> Gamma' Sigma' i' s' a' [] h2 h3 h4; subst.
+Qed.
+
+Lemma type_infer_constu: forall Gamma Sigma ef t, 
+type_expr Gamma Sigma (Const ConsUnit (Ptype Tunit)) ef t ->
+Ptype Tunit = t.
+Proof.
+move=> Gamma Sigma ef t. 
+move eq : (Const ConsUnit (Ptype Tunit))=> v ht. elim: ht eq=>//=.
+Qed.
+
+Lemma type_infer_app: forall Gamma Sigma e es rt ef t,
+type_expr Gamma Sigma (App e es rt) ef t ->
+t = rt.
+Proof.
+move=> Gamma Sigma e es rt ef t.
+move eq: (App e es rt)=> ve ht. elim: ht eq=> //=.
+by move=> Gamma' Sigma' e' es' rt' efs ts ef' efs' ht1 hin ht2 [] h1 h2 h3; subst.
+Qed.
+
+Lemma type_infer_ref: forall Gamma Sigma h bt a e ef t,
+type_expr Gamma Sigma (Prim Ref [:: e] (Reftype h (Bprim bt) a)) ef t ->
+t = (Reftype h (Bprim bt) a).
+Proof.
+move=> Gamma Sigma h bt a e ef t.
+move eq: (Prim Ref [:: e] (Reftype h (Bprim bt) a))=> rv ht.
+elim: ht eq=> //=.
+by move=> Gamma' Sigma' e' ef' h' bt' a' ht hin [] h1 h2 h3 h4; subst.
+Qed.
+
+Lemma type_infer_deref: forall Gamma Sigma bt e ef t,
+type_expr Gamma Sigma (Prim Deref [:: e] (Ptype bt)) ef t ->
+t = (Ptype bt).
+Proof.
+move=> Gamma Sigma bt e ef t.
+move eq: (Prim Deref [:: e] (Ptype bt))=> rv ht.
+elim: ht eq=> //=.
+by move=> Gamma' Sigma' e' ef' h bt' a' ht1 hin1 [] h1 h2; subst.
+Qed.
+
+Lemma type_infer_massgn: forall Gamma Sigma e e' ef t,
+type_expr Gamma Sigma (Prim Massgn [:: e; e'] (Ptype Tunit)) ef t ->
+t = (Ptype Tunit). 
+Proof.
+move=> Gamma Sigma e e' ef t.
+move eq: (Prim Massgn [:: e; e'] (Ptype Tunit))=> rv ht.
+elim: ht eq=> //=.
+Qed.
+
+Lemma type_infer_uop: forall Gamma Sigma e uop t ef' t',
+type_expr Gamma Sigma (Prim (Uop uop) [:: e] t) ef' t' ->
+t' = t.
+Proof.
+move=> Gamma Sigma e uop t ef' t'.
+move eq: (Prim (Uop uop) [:: e] t)=> rv ht.
+elim: ht eq=> //=.
+by move=> Gamma' Sigma' op e' ef t'' hrt hut hte' hin [] h1 h2 h3; subst. 
+Qed.
+
+Lemma type_infer_bop: forall Gamma Sigma e e' t bop ef t',
+type_expr Gamma Sigma (Prim (Bop bop) [:: e; e'] t) ef t' ->
+t' = t.
+Proof.
+move=> Gamma Sigma e e' t bop ef t'.
+move eq: (Prim (Bop bop) [:: e; e'] t)=> rv ht.
+elim: ht eq=> //=.
+by move=> Gamma' Sigma' op e1 ef1 t1 e2 hrt hut ht1 hin1 ht2 hin2
+       [] h1 h2 h3 h4; subst. 
+Qed.
+
+Lemma type_infer_bind: forall Gamma Sigma e x t e' t' ef t'',
+type_expr Gamma Sigma (Bind x t e e' t') ef t'' ->
+t'' = t'.
+Proof.
+move=> Gamma Sigma e x t e' t' ef t''.
+move eq:(Bind x t e e' t')=> rv ht. elim: ht eq=> //=.
+by move=> Gamma' Sigma' x' t1 e1 e2 t2 ef1 ef' ht1 hin ht2 hin'
+       [] h1 h2 h3 h4 h5; subst.
+Qed.
+
+Lemma type_infer_cond: forall Gamma Sigma e1 e2 e3 t ef' t',
+type_expr Gamma Sigma (Cond e1 e2 e3 t) ef' t' ->
+t' = t.
+Proof.
+move=> Gamma Sigma e1 e2 e3 t ef' t'.
+move eq: (Cond e1 e2 e3 t)=> rv ht.
+elim: ht eq=> //=.
+by move=> Gamma' Sigma' e1' e2' e3' tb t1 ef1 ef2 ht1 hin1 htb
+       ht2 hin2 ht3 hin3 [] h1 h2 h3 h4; subst.
+Qed.
+
+Lemma type_infer_unit: forall Gamma Sigma ef t,
+type_expr Gamma Sigma (Unit (Ptype Tunit)) ef t ->
+t = Ptype Tunit.
+Proof.
+move=> Gamma Sigma ef t. move eq: (Unit (Ptype Tunit))=> rv ht.
+by elim: ht eq=> //=.
+Qed.
+
+Lemma type_infer_addr: forall Gamma Sigma l ofs h bt a ef t,
+type_expr Gamma Sigma (Addr l ofs (Reftype h bt a)) ef t ->
+t = (Reftype h bt a).
+Proof.
+move=> Gamma Sigma l ofs h bt a ef t.
+move eq: (Addr l ofs (Reftype h bt a))=> rv ht.
+elim: ht eq=> //=.
+by move=> Gamma' Sigma' l' ofs' h' t' a' hs [] h1 h2 h3 h4 h5; subst.
+Qed.
+
+Lemma type_infer_eapp: forall Gamma Sigma exf es ef t,
+type_expr Gamma Sigma (Eapp exf (get_at_eapp exf) es (get_rt_eapp exf)) ef t ->
+t = (get_rt_eapp exf).
+Proof.
+move=> Gamma Sigma exf es ef t. 
+move eq: (Eapp exf (get_at_eapp exf) es (get_rt_eapp exf))=> rv ht.
+elim: ht eq=> //=.
+by move=> Gamma' Sigma' exf' ts es' ef' rt hrt [] hr1 hr2 hts hes' []
+       h1 h2 h3 h4; subst.
+Qed.
 
 Lemma type_expr_exprs_deterministic: 
 (forall Gamma Sigma es efs ts efs' ts', type_exprs Gamma Sigma es efs ts ->
@@ -265,47 +684,70 @@ Lemma type_expr_exprs_deterministic:
 Proof.
 suff : (forall Gamma Sigma es efs ts, type_exprs Gamma Sigma es efs ts ->
                                       forall efs' ts', type_exprs Gamma Sigma es efs' ts' ->
-                                      ts = ts') /\
+                                                       ts = ts') /\
        (forall Gamma Sigma e ef t, type_expr Gamma Sigma e ef t ->
                                    forall ef' t', type_expr Gamma Sigma e ef' t' ->
-                                   t = t').
+                                                  t = t').
 + move=> [] ih ih'. split=> //=.
   + move=> Gamma Sigma es efs ts efs' ts' hes hes'. 
     by move: (ih Gamma Sigma es efs ts hes efs' ts' hes').
   move=> Gamma Sigma e ef t ef' t' he he'.
   by move: (ih' Gamma Sigma e ef t he ef' t' he').
-apply type_expr_indP => //=.
-+ by move=> Gamma Sigma ef ef' t' ht; inversion ht; subst.
-+ by move=> Gamma Sigma ef i sz s a ef' t' ht; inversion ht; subst.
-+ by move=> Gamma Sigma ef i s a ef' t' ht; inversion ht; subst.
-+ by move=> Gamma Sigma ef l ofs h t a ef' t' hp ht; inversion ht; subst.
-+ move=> Gamma Sigma x t ht ef' t' het; subst. by inversion het; subst.
-+ move=> Gamma Sigma t sz s i a ht ef' t' ht'; subst. by inversion ht'; subst.
-+ move=> Gamma Sigma t s i a ht ef' t' ht'; subst. by inversion ht'; subst.
-+ move=> Gamma Sigma t ht ef' t' ht'; subst. by inversion ht'; subst.
-+ move=> Gamma Sigma e es rt ef efs ts efs' ih ih' ef' t' ht; subst.
-  by inversion ht; subst. 
-+ by move=> Gamma Sigma e ef h bt a ih ef' t' ht; inversion ht; subst.
-+ by move=> Gamma Sigma e ef h bt a ih ef' t' ht; inversion ht; subst.
-+ by move=> Gamma Sigma e1 e2 ef1 ef2 h bt a ih ih' ef' t' ht; inversion ht; subst.
-+ by move=> Gamma Sigma op e ef t hf hf' ih ef' t' ht; inversion ht; subst.
-+ by move=> Gamma Sigma op e1 e2 ef t hf hf' ih ih' ef' t' ht; inversion ht; subst.
-+ by move=> Gamma Sigma x t e e' t' ef ef' ih ih' ef'' t'' ht; inversion ht; subst.
-+ move=> Gamma Sigma e1 e2 e3 ef1 ef2 ef3 tb t ef1' ef hin1 hs1 htb hin3
-  hs2 ht2 hs3 ef' t' htc. by inversion htc; subst.
-+ by move=> Gamma Sigma ef' t' ht; inversion ht; subst.
-+ by move=> Gamma Sigma l ofs h t a hl ef' t'' ht; inversion ht; subst.
-+ by move=> Gamma Sigma exf ts es ef rt hrt [] h1 h2 hts hin ef' t' ht; inversion ht; subst.
-+ by move=> Gamma Sigma efs' ts' ht; inversion ht; subst.
-move=> Gamma Sigma e es t ef ts efs ih ih' efs' ts' ht; inversion ht; subst.
-move: (ih ef0 t0 H3)=> h1; subst. by move: (ih' efs0 ts0 H6)=> h1; subst.
+apply type_exprs_type_expr_ind_mut => //=.
++ move=> Gamma Sigma ef' t' ht; inversion ht; subst; auto.
+  by have := type_infer_vunit Gamma Sigma ef' t' ht.
++ move=> Gamma Sigma i sz s a ef' t' ht; inversion ht; subst; auto.
+  by have := type_infer_int Gamma Sigma ef' t' i sz s a ht.
++ move=> Gamma Sigma i s a ef' t' ht; inversion ht; subst; auto.
+  by have := type_infer_long Gamma Sigma ef' t' i s a ht.
++ move=> Gamma Sigma l ofs h t a hs ef' t' ht; inversion ht; subst; auto.
+  by have := type_infer_loc Gamma Sigma ef' t' h t a l ofs ht.
++ move=> Gamma Sigma x t ht ef' t' ht'; subst; inversion ht'; subst; auto.
+  by have := type_infer_var Gamma Sigma x t ef' t' ht'.
++ move=> Gamma Sigma sz s a i ef' t' ht; subst; inversion ht; subst; auto.
+  by have := type_infer_consti Gamma Sigma ef' t' i sz s a ht.
++ move=> Gamma Sigma s a i ef' t' ht; subst; inversion ht; subst; auto.
+  by have := type_infer_constl Gamma Sigma ef' t' i s a ht.
++ move=> Gamma Sigma ef' t' ht; inversion ht; subst; auto.
+  by have := type_infer_constu Gamma Sigma ef' t' ht.
++ move=> Gamma Sigma e es rt efs ts ef efs' hte hin htes hin' ef' t ht; 
+  inversion ht; subst; auto.
+  by have := type_infer_app Gamma Sigma e es rt ef' t ht.
++ move=> Gamma Sigma e ef h bt a hte hin ef' t' ht; inversion ht; subst; auto.
+  by have := type_infer_ref Gamma Sigma h bt a e ef' t' ht.
++ move=> Gamma Sigma e ef h bt a hte ef' ef'' t' ht; inversion ht; subst; auto.
+  by have := type_infer_deref Gamma Sigma bt e ef'' t' ht.
++ move=> Gamma Sigma e e' h bt ef a ef' hte hin hte' hin' ef'' t' ht; subst; auto.
+  by have := type_infer_massgn Gamma Sigma e e' ef'' t' ht.
++ move=> Gamma Sigma op e ef t hrt hut hte hin ef' t' ht; inversion ht; subst; auto.
+  by have := type_infer_uop Gamma Sigma e op t ef' t' ht.
++ move=> Gamma Sigma op e ef t e' hrt hut hte hin hte' hin' 
+  ef' t' ht; inversion ht; subst; auto.
+  by have := type_infer_bop Gamma Sigma e e' t op ef' t' ht.
++ move=> Gamma Sigma x t e e' t' ef ef' hte hin hte' hin' ef'' t'' ht; 
+  inversion ht; subst; auto.
+  by have := type_infer_bind Gamma Sigma e x t e' t' ef'' t'' ht.
++ move=> Gamma Sigma e1 e2 e3 tb t ef1 ef2 hte1 hin1 htb hte2 hin2 hte3 hin3 ef' t'
+         ht; inversion ht; subst; auto.
+  by have := type_infer_cond Gamma Sigma e1 e2 e3 t ef' t' ht.
++ move=> Gamma Sigma ef' t' ht; inversion ht; subst; auto.
+  by have := type_infer_unit Gamma Sigma ef' t' ht.
++ move=> Gamma Sigma l ofs h t a hs ef' t' ht; inversion ht; subst; auto.
+  by have := type_infer_addr Gamma Sigma l ofs h t a ef' t' ht.
++ move=> Gamma Sigma exf ts es ef rt hrt [] h1 h2 h3 ht1 hin ef' t' ht; subst;
+         inversion ht; subst; auto.
+  by have := type_infer_eapp Gamma Sigma exf es ef' t' ht.
++ by move=> Gamma Sigma efs' ts' ht; inversion ht; subst; auto.
+move=> Gamma Sigma e es ef efs t ts hte hin htes hin' efs' ts' ht;
+       inversion ht; subst; auto.
+move: (hin ef0 t0 H3)=> ->. by move: (hin' efs0 ts0 H6)=> ->.
 Qed.
 
 Lemma type_rel_typeof : forall Gamma Sigma e ef t,
 type_expr Gamma Sigma e ef t ->
 typeof_expr e = t.
 Proof.
-by move=> Gamma Sigma e ef t ht; inversion ht; subst; rewrite /typeof_expr /=; auto.
+by move=> Gamma Sigma e ef t ht; elim: ht=> //=.
 Qed.
 
 Lemma eq_type_rel : forall v t t',
@@ -402,27 +844,6 @@ Proof.
 move=> v chunk v'. case: chunk=> //=; case: v=> //=; case: v'=> //=. 
 Admitted.
 
-(* Value typing *)
-(* A value does not produce any effect *)
-Lemma value_typing : forall Gamma Sigma ef t v,
-type_expr Gamma Sigma (Val v t) ef t ->
-type_expr Gamma Sigma (Val v t) empty_effect t. 
-Proof.
-move=> Gamma Sigma ef t v ht. inversion ht.
-+ by apply ty_valu.
-+ by apply ty_vali.
-+ by apply ty_vall.
-by apply ty_valloc.  
-Qed.
-
-(* Value type same *)
-Lemma type_val_reflx : forall Gamma Sigma v t ef t',
-type_expr Gamma Sigma (Val v t) ef t' -> 
-t = t'.
-Proof.
-move=> Gamma Sigma v t ef t' ht. by inversion ht; subst.
-Qed.
-
 
 (* Complete Me: Easy *)
 (* There always exists a C type for BeePL type which is 
@@ -434,15 +855,5 @@ Lemma well_typed_success:
                             exists ct g i, transBeePL_type t g = Res ct g i).
 Proof.
 apply type_exprs_type_expr_ind_mut=> //=.
-+ move=> Gamma Sigma ef. exists Tvoid. eexists. by eexists.
-+ move=> Gamma Sigma ef i sz s a. exists (Ctypes.Tint sz s a). eexists. by eexists.
-+ move=> Gamma Sigma ef l s a. exists (Ctypes.Tlong s a). eexists. by eexists.
-+ move=> Gamma Sigma ef l ofs h t a. case: t=> //= p. case: p=> //=.
-  + exists (Tpointer Tvoid a). eexists. by eexists.
-  + move=> sz s a'. exists (Tpointer (Ctypes.Tint sz s a') a). eexists. by eexists.
-  move=> s a'. exists (Tpointer (Ctypes.Tlong s a') a). eexists. by eexists.
-+ move=> Gamma Sigma x t ht. case: t ht=> //=.
-  + move=> p. case: p=> //=.
-    + exists Tvoid.
 Admitted.
 
